examples/opaque: add subterm lemmas

examples/opaque/shared.v
@@ -198,3 +198,517 @@ by solve_ndisj.
 Qed.
 
 End Opaque.
+
+Lemma subterm_of_list (t : term) (ts : list term) :
+  (exists t', t' ∈ ts /\ subterm t t')  ->
+  subterm t (Spec.of_list ts).
+Proof.
+  intros [t' [Hmem Hsubterm]].
+  induction ts.
+  by inversion Hmem.
+  rewrite elem_of_cons in Hmem.
+  rewrite Spec.of_list_unseal.
+  simpl.
+  destruct Hmem as [Hmem|Hmem].
+  subst.
+  by apply STPair1.
+  apply STPair2.
+  rewrite -Spec.of_list_unseal.
+  by apply IHts.
+Qed.
+
+Lemma subterm_of_tag (t t' : term) (n : namespace) :
+  subterm t t' ->
+  subterm t (Spec.tag (Tag n) t').
+Proof.
+  intro.
+  rewrite Spec.tag_unseal.
+  by apply STPair2.
+Qed.
+
+Lemma subterm_TExpN_exp (t t' : term) (ts : list term) :
+  ( exists t'', subterm t t'' /\ t'' ∈ ts) ->
+  negb (is_exp t') ->
+  invs_canceled ts ->
+  subterm t (TExpN t' ts).
+Proof.
+  intros [t'' [Hst Hmem]] Hnexp Hcanceled.
+  by apply (STExp2 Hnexp Hcanceled Hst Hmem).
+Qed.
+
+Lemma subterm_TExp_exp (t t' t'' : term) :
+  negb (is_exp t') ->
+  subterm t t'' ->
+  subterm t (TExp t' t'').
+Proof.
+  intros Hnexp Hst.
+  apply subterm_TExpN_exp => //.
+  exists t''. split => //.
+  rewrite elem_of_cons.
+  by left.
+  by apply invs_canceled1.
+Qed.
+
+Lemma andb_is_true b1 b2:
+  is_true (b1 && b2) <-> is_true b1 /\ is_true b2.
+Proof.
+  by rewrite /is_true andb_true_iff.
+Qed.
+
+
+Lemma map_cancel_if {T : Type} (P : ssrbool.pred T) (f : T -> T)
+                 (H : forall x, is_true (P x) -> f x = x) :
+  forall l, seq.all P l -> seq.map f l = l.
+Proof.
+  intros l.
+  induction l => H' //=.
+  rewrite /= andb_True in H'.
+  destruct H' as [H' H''].
+  rewrite -is_trueP in H'.
+  f_equal => //.
+  by apply H.
+  by apply IHl.
+Qed.
+
+Lemma map_compose {T T' T'' : Type} (f : T -> T') (f' : T' -> T'') (f'' : T -> T'')
+                  (H : forall x, f' (f x) = f'' x) :
+  forall l, seq.map f' (seq.map f l) = seq.map f'' l.
+Proof.
+  intros l.
+  induction l => //=.
+  by f_equal.
+Qed.
+
+Definition normalize_wfs := map_cancel_if PreTerm.normalize_wf.
+
+Definition map_unfold_fold := map_compose unfold_fold.
+
+(* unused: for completeness *)
+Definition map_fold_termK := map_cancel_if fold_termK.
+
+Lemma map_wf_unfold_fold (pts : list PreTerm.pre_term) :
+  is_true (seq.all PreTerm.wf_term pts) ->
+  seq.map unfold_term (seq.map fold_term pts) = pts.
+Proof.
+  intro H.
+  by rewrite map_unfold_fold normalize_wfs // H.
+Qed.
+
+(* Definition propositional_extensionality : Prop := *)
+(*   forall (P Q : Prop), (P <-> Q) -> P = Q. *)
+
+Definition proof_irrelevance : Prop :=
+  forall (P : Prop) (pf1 pf2 : P), pf1 = pf2.
+
+Lemma TExpN'_TExpN (pt : PreTerm.pre_term) (pts : list PreTerm.pre_term) i :
+  proof_irrelevance ->
+  TExpN' pt pts i = TExpN (fold_term pt) (seq.map fold_term pts).
+Proof.
+  intro Hpi.
+  rewrite /TExpN unlock.
+  specialize i as i'.
+  rewrite /= !andb_is_true in i'.
+  destruct i' as [Hwf [Hnexp [Hwfs [Hnempty [Hsorted Hcanceled]]]]].
+  apply ssrbool.negbTE in Hnexp.
+  apply ssrbool.negbTE in Hnempty.
+  rewrite map_wf_unfold_fold // /PreTerm.exp !unfold_fold !PreTerm.normalize_wf => //.
+  destruct pt; try by inversion Hnexp.
+  1- 3: rewrite /PreTerm.exps /= PreTerm.cancel_exps_canceled // path.sorted_sort //;
+                try apply preorder.Order.PreorderTheory.le_trans;
+  rewrite -seq.nilpE in Hnempty;
+  rewrite Hnempty unlock /fold_term_def PreTerm.normalize_wf // /fold_term_predef;
+  rewrite seq.nilpE in Hnempty;
+  set b := ssrbool.boolP _;
+          destruct b;
+          f_equal.
+  1, 3, 5: by apply Hpi.
+  all: by rewrite i /is_true /= in i0.
+Qed.
+
+Definition map_unfold_termK := seq.mapK unfold_termK.
+
+Lemma map_nil {T T' : Type} (l : list T) (f : T -> T') :
+seq.map f l = [] <-> l = [].
+Proof.
+  by split; intro; destruct l.
+Qed.
+
+Lemma map_nnil {T T' : Type} (l : list T) (f : T -> T') :
+seq.map f l ≠ [] <-> l ≠ [].
+Proof.
+  by rewrite map_nil.
+Qed.
+
+Lemma nilp_sort {T : Type} f (l : list T) :
+  seq.nilp (path.sort f l) = seq.nilp l.
+Proof.
+  by rewrite /seq.nilp path.size_sort.
+Qed.
+
+(* could be useful, but not necessary for this *)
+(* Lemma cancel_exps_sort l : *)
+(*   path.sort preorder.Order.le (PreTerm.cancel_exps l) *)
+(*   = PreTerm.cancel_exps (path.sort preorder.Order.le l). *)
+(* Admitted. *)
+
+Lemma unfold_cancel_exps l:
+  seq.map unfold_term (cancel_exps l) = PreTerm.cancel_exps (seq.map unfold_term l).
+Proof.
+  by rewrite /cancel_exps map_wf_unfold_fold // PreTerm.wf_cancel_exps // wf_unfold_terms.
+Qed.
+
+Lemma nilp_false (ts : list PreTerm.pre_term) :
+  ts ≠ [] ->
+  seq.nilp ts = false.
+Proof.
+  intro contra.
+  by destruct ts.
+Qed.
+
+Lemma TExpN_TExpN' (t : term) (ts : list term) :
+  proof_irrelevance ->
+  is_true (negb (is_exp t)) ->
+  cancel_exps ts ≠ [] ->
+  exists i,
+    TExpN t ts =
+      TExpN' (unfold_term t) (path.sort preorder.Order.le (seq.map unfold_term (cancel_exps ts))) i.
+Proof.
+  intros Hpi Hnexp Hnnil.
+  rewrite unfold_cancel_exps.
+  assert (is_true (PreTerm.wf_term
+                     (PreTerm.PTExp
+                        (unfold_term t)
+                        (path.sort preorder.Order.le (PreTerm.cancel_exps (seq.map unfold_term ts))))))
+    as i. {
+    rewrite /= !andb_is_true wf_unfold_term path.all_sort -is_exp_unfold (path.sort_sorted order.Order.TotalTheory.le_total).
+    do !split => //.
+       by rewrite PreTerm.wf_cancel_exps // wf_unfold_terms.
+       rewrite -seq.size_eq0 path.size_sort -unfold_cancel_exps seq.size_map.
+       by destruct (cancel_exps ts).
+       by rewrite -unfold_cancel_exps PreTerm.invs_canceled_sort /cancel_exps
+                                      map_wf_unfold_fold ?PreTerm.invs_canceled_cancel_exps
+                                      // ?PreTerm.wf_cancel_exps // wf_unfold_terms.
+  }
+  exists i.
+  assert (forall l, seq.cat (PreTerm.exps (unfold_term t)) l = l) as H. {
+    rewrite PreTerm.exps_expN //=.
+    by rewrite -is_exp_unfold.
+  }
+  rewrite !unlock /fold_term_def /PreTerm.exp H. 
+  rewrite /cancel_exps map_nnil in Hnnil.
+  specialize (nilp_false Hnnil) as Hnnil'.
+  rewrite Hnnil' -unfold_base base.base_expN //= normalize_unfold1 normalize_wfs.
+  2: by rewrite path.all_sort -is_trueP;
+  apply PreTerm.wf_cancel_exps;
+  apply wf_unfold_terms.
+  rewrite /PreTerm.exp H PreTerm.cancel_exps_canceled.
+  2: by rewrite PreTerm.invs_canceled_sort PreTerm.invs_canceled_cancel_exps //;
+                apply wf_unfold_terms.
+  rewrite nilp_sort Hnnil' (path.sorted_sort order.Order.POrderTheory.le_trans).
+  2: by rewrite (path.sort_sorted order.Order.TotalTheory.le_total).
+  rewrite -unfold_base base.base_expN // /fold_term_predef.
+  set b := ssrbool.boolP _;
+          destruct b.
+  by f_equal.
+  by rewrite i in i0.
+Qed.
+
+(* Lemma eqtype_eq (l l' : list PreTerm.pre_term) : *)
+(*   @eqtype.eq_op *)
+(*     (seq.Datatypes_list__canonical__eqtype_Equality *)
+(*        PreTerm.PreTerm_pre_term__canonical__eqtype_Equality) *)
+(*     l l' = true <-> l = l'. *)
+(* Proof. *)
+(*   generalize l'. *)
+(*   clear l'. *)
+(*   induction l => l'; destruct l';  *)
+(*                 rewrite // seq.eqseq_cons andb_true_iff; *)
+(*                 split => H //. *)
+(*   destruct H as [H H']. *)
+(*   f_equal. *)
+(*   admit. *)
+(*   by apply IHl. *)
+(*   inversion H. *)
+(*   by split; apply eqtype.eq_refl. *)
+(* Admitted. *)
+
+Lemma eqtype_eq_nil (l : list PreTerm.pre_term) :
+  @eqtype.eq_op
+    (seq.Datatypes_list__canonical__eqtype_Equality
+       PreTerm.PreTerm_pre_term__canonical__eqtype_Equality)
+    l [] = true <-> l = [].
+Proof.
+  by destruct l.
+Qed.
+
+Lemma eqtype_sort_nil f (l : list PreTerm.pre_term) :
+  @eqtype.eq_op
+    (seq.Datatypes_list__canonical__eqtype_Equality
+       PreTerm.PreTerm_pre_term__canonical__eqtype_Equality)
+    (path.sort f l) [] =
+    @eqtype.eq_op
+      (seq.Datatypes_list__canonical__eqtype_Equality
+         PreTerm.PreTerm_pre_term__canonical__eqtype_Equality)
+      l [].
+Proof.
+  by rewrite -!seq.nilpE nilp_sort.
+Qed.
+
+Lemma TExpN_inj (t t' : term) (ts ts' : list term) :
+  proof_irrelevance ->
+  is_true (negb (is_exp t)) ->
+  is_true (negb (is_exp t')) ->
+  TExpN t ts = TExpN t' ts' ->
+  t = t'.
+Proof.
+  intros Hpi Hnexp Hnexp' Heq.
+  destruct (list_eq_nil_dec (cancel_exps ts)) as [Hncan | Hncan'].
+  destruct (list_eq_nil_dec (cancel_exps ts')) as [Hncan' | Hncan'].
+  3: destruct (list_eq_nil_dec (cancel_exps ts')) as [Hncan | Hncan].
+  1- 3: rewrite /cancel_exps !map_nil in Hncan Hncan'.
+  by rewrite /TExpN unlock /PreTerm.exp -!unfold_exps !base.exps_expN //=
+             Hncan Hncan' /= -!unfold_base !base.base_expN // !unfold_termK in Heq.
+  1, 2: rewrite /TExpN unlock /PreTerm.exp -!unfold_exps !base.exps_expN //=
+                Hncan /= (nilp_false Hncan') -!unfold_base !base.base_expN //
+                unfold_termK /= /fold_term unlock /fold_term_def /=
+                normalize_unfold1 /PreTerm.exp -!unfold_exps
+                !base.exps_expN //= normalize_wfs in Heq.
+  2, 4: by rewrite path.all_sort PreTerm.wf_cancel_exps // wf_unfold_terms.
+  1, 2: rewrite PreTerm.cancel_exps_canceled in Heq.
+  2, 4: by rewrite PreTerm.invs_canceled_sort PreTerm.invs_canceled_cancel_exps //
+                   wf_unfold_terms.
+  1, 2: rewrite (path.sorted_sort
+                   order.Order.POrderTheory.le_trans
+                   (path.sort_sorted
+                      order.Order.TotalTheory.le_total
+                      (PreTerm.cancel_exps (seq.map unfold_term _))))
+                nilp_sort nilp_false // -!unfold_base !base.base_expN //
+                /fold_term_predef in Heq;
+  set b := ssrbool.boolP _ in Heq;
+          destruct b.
+  by rewrite Heq in Hnexp.
+  2: by rewrite -Heq in Hnexp'.
+  1, 2: rewrite /= /is_true negb_true_iff !andb_false_iff in i;
+  destruct i as [contra' | [contra' | [contra' | [contra' | [contra' | contra']]]]].
+  1, 7: by rewrite wf_unfold_term in contra'.
+  1, 6: by rewrite -is_exp_unfold ?Hnexp' ?Hnexp in contra'.
+  1, 5: by rewrite path.all_sort PreTerm.wf_cancel_exps // wf_unfold_terms in contra'.
+  1, 4: by destruct Hncan';
+  rewrite negb_false_iff eqtype_sort_nil eqtype_eq_nil in contra'.
+  1, 3: by rewrite (path.sort_sorted order.Order.TotalTheory.le_total) in contra'.
+  1, 2: by rewrite PreTerm.invs_canceled_sort PreTerm.invs_canceled_cancel_exps //
+                   wf_unfold_terms in contra'.
+  destruct (TExpN_TExpN' Hpi Hnexp Hncan') as [i H].
+  destruct (TExpN_TExpN' Hpi Hnexp' Hncan) as [i' H'].
+  rewrite H H' // in Heq.
+  inversion Heq.
+  by apply unfold_term_inj in H1.
+Qed.
+
+Lemma is_exp_fold pt :
+  is_true (PreTerm.wf_term pt) ->
+  PreTerm.is_exp pt = is_exp (fold_term pt).
+Proof.
+  intro Hwf.
+  rewrite /is_exp /fold_term /PreTerm.is_exp unlock /fold_term_def /fold_term_predef
+           PreTerm.normalize_wf ?Hwf //.
+  destruct pt => //.
+  1-3: destruct t => //.
+  all: set b := ssrbool.boolP _;
+               destruct b => //.
+  by rewrite Hwf in i.
+Qed. 
+
+Lemma elem_of_sorted_terms t ts :
+  t ∈ ts <-> t ∈ seq.map fold_term (path.sort preorder.Order.le (seq.map unfold_term ts)).
+Proof.
+  by rewrite !(ssrbool.rwP inP) path.sort_map map_unfold_termK path.mem_sort.
+Qed.
+
+Lemma TInv_TInv' t:
+  proof_irrelevance ->
+  is_true (negb (is_inv t)) ->
+  exists i, TInv t = TInv' (unfold_term t) i.
+Proof.
+  intros Hpi H.
+  assert (is_true (PreTerm.wf_term (PreTerm.PT1 O1Inv (unfold_term t)))) as i. {
+    rewrite /= andb_is_true -is_inv_unfold wf_unfold_term.
+    by split.
+  }
+  exists i.
+  rewrite /TInv unlock /PreTerm.inv.
+  rewrite is_inv_unfold in H.
+  destruct (unfold_term t).
+  2: destruct t0.
+  all: by rewrite /fold_term unlock /fold_term_def PreTerm.normalize_wf //
+                  /fold_term_predef;
+    set b := ssrbool.boolP _;
+            destruct b;
+            f_equal => //;
+                        rewrite i in i0.
+Qed.
+
+(* unused: for completeness *)
+Lemma TInv'_TInv (pt : PreTerm.pre_term) i :
+  proof_irrelevance ->
+  TInv' pt i = TInv (fold_term pt).
+Proof.
+  intro Hpi.
+  specialize i as i'.
+  rewrite /= !andb_is_true in i'.
+  destruct i' as [Hninv Hwf].
+  set t := fold_term pt.
+  assert (pt = unfold_term t) as Heq. {
+    by rewrite /t unfold_fold (PreTerm.normalize_wf Hwf).
+  }
+  rewrite Heq -is_inv_unfold in Hninv.
+  generalize i.
+  rewrite Heq.
+  intro i'.
+  destruct (TInv_TInv' Hpi Hninv) as [i'' H].
+  rewrite H /t.
+  by f_equal.
+Qed.
+
+Lemma subterm_exp (t t' : term) :
+  proof_irrelevance ->
+  t ≠ t' ->
+  subterm t t' <-> subterm t (base t') \/ exists t'', subterm t t'' /\ t'' ∈ exps t'.
+Proof.
+  intros Hpi Hneq.
+  split; intros H; destruct t'; try by left.
+  simpl.
+  rewrite TExpN'_TExpN in Hneq H => //.
+  inversion H.
+  by destruct Hneq.
+  1, 2, 3, 4, 5, 6: rewrite -TExpN'_TExpN in H0 => //; inversion H0.
+  rewrite -TExpN'_TExpN in H0 => //.
+  rewrite -is_trueP in H1.
+  destruct (TInv_TInv' Hpi H1) as [i' H'].
+  rewrite H' in H0.
+  inversion H0.
+  assert (t' = fold_term pt) as H'. {
+    rewrite /= !andb_is_true in i.
+    destruct i as [Hwf [Hnexp [Hwfs [Hnnil [Hsort Hcan]]]]].
+    rewrite (is_exp_fold Hwf) in Hnexp.
+    rewrite -is_trueP in H1.
+    specialize TExpN_inj as i.
+    apply (i t' (fold_term pt) ts (seq.map fold_term pts)) => //.
+  }
+  subst.
+  by left.
+  rewrite -TExpN'_TExpN in H0 => //.
+  rewrite -is_trueP in H1.
+  assert (ts ≠ []) as Hnnil. {
+    destruct ts => //.
+    by inversion H4.
+  }
+  rewrite -(cancel_exps_canceled H2) in Hnnil.
+  destruct (TExpN_TExpN' Hpi H1 Hnnil) as [i' eqv].
+  rewrite eqv in H0.
+  inversion H0.
+  right.
+  exists t''.
+  split => //.
+  by rewrite (cancel_exps_canceled H2) -elem_of_sorted_terms.
+  1- 7: by destruct H => //; destruct H as [t'' [_ contra]]; destruct (not_elem_of_nil t'').
+  rewrite TExpN'_TExpN //.
+  simpl in H.
+  destruct H.
+  apply STExp1 => //.
+  clear Hneq.
+  rewrite /= !andb_is_true in i.
+  destruct i as [H' [i _]].
+  by rewrite is_exp_unfold unfold_fold PreTerm.normalize_wf ?i.
+  clear Hneq.
+  rewrite /= !andb_is_true in i.
+  destruct i as [Hwf [Hnexp [Hwfs [_ [_ Hcanceled]]]]].
+  apply subterm_TExpN_exp => //.
+  by rewrite is_exp_unfold unfold_fold PreTerm.normalize_wf // Hnexp.
+  by rewrite /invs_canceled map_wf_unfold_fold // Hcanceled.
+Qed.
+
+(* Lemma term_preterm_mem_eq (t : term) (ts : list term) : *)
+(* ssrbool.in_mem t (ssrbool.mem ts) *)
+(* = ssrbool.in_mem (unfold_term t) (ssrbool.mem (seq.map unfold_term ts)). *)
+(* Admitted. *)
+
+Lemma cons_invs_canceled t ts :
+  ¬ (TInv t ∈ ts) ->
+  invs_canceled ts ->
+  cancel_exps (t :: ts) = t :: ts.
+Proof.
+  intros Hfresh Hcan.
+  rewrite cancel_exps_canceled // invs_canceled_cons.
+  by split.
+Qed.
+
+Lemma subterm_TExp_exp' (t t' t'' : term) :
+  proof_irrelevance ->
+  ¬ subterm t t' ->
+  ¬ subterm t'' t' ->
+  negb (is_inv t'') ->
+  subterm t t'' ->
+  subterm t (TExp t' t'').
+Proof.
+  intros Hpi Hnst Hnst' Hninv Hst.
+  destruct (term_eq_dec t (TExp t' t'')).
+  by rewrite e.
+  destruct (is_exp t') eqn:E.
+  rewrite (subterm_exp Hpi n).
+  right.
+  assert (exps (TExp t' t'') =
+            (seq.map fold_term (path.sort preorder.Order.le (seq.map unfold_term (t'' :: exps t')))))
+    as H. {
+    destruct t'; try by inversion E.
+    set pt'' := unfold_term t''.
+    assert (t'' = fold_term pt'').
+    by rewrite /pt'' unfold_termK.
+    rewrite TExpN'_TExpN // TExp_TExpN H -seq.map_cons // path.sort_map map_unfold_termK.
+    specialize i as i'.
+    rewrite /= !andb_is_true in i'.
+    destruct i' as [Hwf [Hnexp [Hwfs [Hnnil [Hsorted Hcan]]]]].
+    rewrite (is_exp_fold Hwf) in Hnexp.
+    assert (cancel_exps (seq.map fold_term (pt'' :: pts)) ≠ []) as H'. {
+      rewrite /= cons_invs_canceled.
+      by intro contra.
+      rewrite -H.
+      intro contra.
+      destruct Hnst'.
+      rewrite TExpN'_TExpN //.
+      apply subterm_TExpN_exp.
+      exists (TInv t'').
+      split => //.
+      by apply STInv.
+      specialize i as i'.
+      rewrite /= !andb_is_true in i'.
+      destruct i' as [Hwf' [Hnexp' _]].
+      by rewrite is_exp_unfold unfold_fold (PreTerm.normalize_wf Hwf') Hnexp'.
+      all: by rewrite /invs_canceled (map_wf_unfold_fold Hwfs) Hcan.
+    }
+    destruct (TExpN_TExpN' Hpi Hnexp H') as [i' H''].
+    rewrite H'' -TExpN'_TExpN // /= path.sort_map map_unfold_termK.
+    f_equal.
+    rewrite cons_invs_canceled => //.
+    intro contra.
+    destruct Hnst'.
+    rewrite TExpN'_TExpN //.
+    apply subterm_TExpN_exp.
+    exists (TInv t'').
+    split => //.
+    by apply STInv.
+    by rewrite H.
+    specialize i as i''.
+    rewrite /= !andb_is_true in i''.
+    destruct i'' as [Hwf' [Hnexp' _]].
+    by rewrite is_exp_unfold unfold_fold (PreTerm.normalize_wf Hwf') Hnexp'.
+    all: by rewrite /invs_canceled (map_wf_unfold_fold Hwfs) Hcan.
+  }
+  rewrite H.
+  exists t''.
+  split => //.
+  rewrite -elem_of_sorted_terms elem_of_cons.
+  by left.
+  apply subterm_TExp_exp => //.
+  by rewrite E.
+Qed.
